\documentclass{article}
\usepackage{mathabx}
\title{null}
\author{null}
\begin{document}
	\maketitle
	$$\lambda_l=\frac{\mu_{n-l}}{\mu_{n+1-l}}$$
	$$\lambda_l $$
	\begin{equation}
	b_l=\frac{\mu_{n-l}}{\mu_{n+1-l}} a_l+(1-\frac{\mu_{n-l}}{\mu_{n+1-l}})d_l
	\end{equation}
	
	\begin{equation}
	c_l=(1-\frac{\mu_{n-l}}{\mu_{n+1-l}}) a_l+(\frac{\mu_{n-l}}{\mu_{n+1-l}})d_l
	\end{equation}
	
	$$(\lambda+1)$$\newline
	$$\lambda_{l+1}=\frac{\mu_{n-1-l}}{\mu_{n-l}}$$
	$$\bar{f_k}(b_l)>\bar{f_k}(c_l)$$
	$$[b_l,d_l]$$
	$$a_{l+1}=b_l$$
	$$d_{l+1}=d_l$$
	$$b_{l+1}=\lambda_{l+1}a_{l+1}+(1-\lambda_{l+1})d_{l+1}$$
	$$c_{l+1}=(1-\lambda_{l+1})a_{l+1}+\lambda_{l+1}d_{l+1}$$
	$$a_{l+1}$$
	$$b_l$$
	
	$$
	b_{l+1}=\lambda_{l+1} b_l+(1-\lambda_{l+1})d_l=\frac{\mu_{n-1-l}}{\mu_{n-l}}(\frac{\mu_{n-l}}{\mu_{n+1-l}}a_l+(1-\frac{\mu_{n-l}}{\mu_{n+1-l}})d_l)+(1-\frac{\mu_{n-l}}{\mu_{n+1-l}})d_l$$ $$\newline\centering \rightarrow b_{l+1}=\frac{\mu_{n-1-l}}{\mu_{n+1-l}} a_l+(1-\frac{\mu_{n-1-l}}{\mu_{n+1-l}})d_l
	$$
	$$\mu_{n+1-l}=\mu_{n-l}+\mu_{n-1-l}$$
	$$b_l$$
	\begin{equation}
	b_{l+1}=\frac{\mu_{n+1-l}-\mu_{n-l}}{\mu_{n+1-l}}a_l+\frac{\mu_{n-l}}{\mu_{n+1-l}} d_l=(1-\frac{\mu_{n-l}}{\mu_{n+1-l}})a_l+\frac{\mu_{n-l}}{\mu_{n+1-l}}d_l=c_l
	\end{equation}
		$$\bar{f_k}(b_l)<\bar{f_k}(c_l)$$
		$$a_{l+1}=a_l,d_{l+1}=c_l$$
		$$c_{l+1}=b_l$$
\end{document}